NLustre/Stream.v
@@ -229,6 +229,61 @@ if the clocked stream is [absent] at the corresponding instant. *)
     intro; discriminate.
   Qed.
 
+  Definition absent_list (xs: list value): Prop :=
+    Forall (fun v => v = absent) xs.
+
+  Definition present_list (xs: list value): Prop :=
+    Forall (fun v => v <> absent) xs.
+
+  Definition all_absent {A} (l: list A) : list value :=
+    map (fun _ => absent) l.
+
+  Remark all_absent_spec:
+    forall A (l: list A),
+      absent_list (all_absent l).
+  Proof.
+    induction l; simpl; constructor; auto.
+  Qed.
+
+  Remark nth_all_absent:
+    forall (xs: list value) n,
+      nth n (all_absent xs) absent = absent.
+  Proof.
+    induction xs, n; simpl; auto.
+  Qed.
+
+  Lemma absent_list_spec:
+    forall xs,
+      absent_list xs <-> xs = all_absent xs.
+  Proof.
+    induction xs; simpl; split; intro; try constructor(auto).
+    - inv H. apply f_equal. now apply IHxs.
+    - now inversion H.
+    - inversion H. rewrite <- H2. now apply IHxs.
+  Qed.
+
+  Lemma present_list_spec:
+    forall xs,
+      present_list xs <-> exists (vs: list val), xs = map present vs.
+  Proof.
+    induction xs as [| x xs IHxs].
+    - split; intro H.
+      + exists []; eauto.
+      + constructor.
+    - split; intro H.
+      + inversion H as [| ? ? Hx Hxs]; subst.
+        apply not_absent_present in Hx as [v Hv].
+        apply IHxs in Hxs as [vs Hvs].
+        exists (v :: vs). simpl.
+        congruence.
+      + destruct H as [vs Hvs].
+        destruct vs; simpl; try discriminate.
+        apply Forall_cons.
+        * intro. subst x; discriminate.
+        * eapply IHxs.
+          exists vs. now inv Hvs.
+  Qed.
+
 End STREAM.
 
 Module StreamFun
